ffi/ByteStringFFI.v
@@ -14,11 +14,11 @@ Require Import
   ByteString.ByteStringHeap
   Coq.FSets.FMapFacts
   Coq.Structures.DecidableTypeEx
+  Coq.Strings.String
   Hask.Data.Functor
   Hask.Control.Monad
   Hask.Control.Monad.Trans.FiatState
   Hask.Control.Monad.Free.
-
 
 (****************************************************************************
  * Compile [buffer_cons] into a [ClientDSL] term
@@ -40,6 +40,7 @@ Definition buffer_empty :=
 
 Hint Unfold buffer_empty.
 
+Check "Compiling emptyDSL...".
 Definition emptyDSL : reflect_ADT_DSL_computation HeapSpec buffer_empty.
 Proof.
   Time compile_term.
@@ -57,16 +58,16 @@ Hint Unfold HeapState.find_free_block.
 Hint Unfold ByteStringHeap.buffer_pack_obligation_1.
 Hint Unfold buffer_pack.
 
+Check "Compiling packDSL...".
 Definition packDSL h xs:
   reflect_ADT_DSL_computation HeapSpec (buffer_pack xs h).
 Proof.
   Local Opaque alloc.
   Local Opaque write.
   Time compile_term.
-    admit.
   Local Transparent alloc.
   Local Transparent write.
-Admitted.
+Defined.
 
 Corollary packDSL_correct : forall (h : Rep HeapSpec) xs,
   refine (buffer_pack xs h)
@@ -75,6 +76,7 @@ Proof. intros; apply denote_refineEquiv. Qed.
 
 Hint Unfold buffer_unpack.
 
+Check "Compiling unpackDSL...".
 Definition unpackDSL h bs:
   reflect_ADT_DSL_computation HeapSpec (buffer_unpack bs h).
 Proof.
@@ -95,6 +97,7 @@ Hint Unfold ByteStringHeap.buffer_cons_obligation_3.
 Hint Unfold poke_at_offset.
 Hint Unfold buffer_cons.
 
+Check "Compiling consDSL...".
 Definition consDSL r ps w :
   reflect_ADT_DSL_computation HeapSpec (buffer_cons (r, ps) w).
 Proof.
@@ -118,6 +121,7 @@ Proof. intros; apply denote_refineEquiv. Qed.
 
 Hint Unfold buffer_uncons.
 
+Check "Compiling unconsDSL...".
 Definition unconsDSL r ps:
   reflect_ADT_DSL_computation HeapSpec (buffer_uncons (r, ps)).
 Proof.
@@ -142,6 +146,7 @@ Proof. intros; apply denote_refineEquiv. Qed.
 Hint Unfold ByteStringHeap.buffer_append_obligation_1.
 Hint Unfold buffer_append.
 
+Check "Compiling appendDSL...".
 Definition appendDSL r1 ps1 ps2:
   reflect_ADT_DSL_computation HeapSpec (buffer_append (r1, ps1) (r1, ps2)).
 Proof.
@@ -163,317 +168,4 @@ Corollary appendDSL_correct : forall (r1 : Rep HeapSpec) (bs1 bs2 : PS),
          (denote HeapSpec (projT1 (appendDSL r1 bs1 bs2))).
 Proof. intros; apply denote_refineEquiv. Qed.
 
-(****************************************************************************
- * Denote a [ClientDSL HeapSpec] term into a GHC computation
- ****************************************************************************)
-
-Axiom IO : Type -> Type.
-
-Axiom fmapIO   : forall {a b : Type}, (a -> b) -> IO a -> IO b.
-Axiom bindIO   : forall {a b : Type}, IO a -> (a -> IO b) -> IO b.
-Axiom returnIO : forall {a : Type}, a -> IO a.
-Axiom failIO   : forall {a : Type}, IO a.
-Axiom joinIO   : forall {a : Type}, IO (IO a) -> IO a.
-
-Axiom bindIO_returnIO : forall {a b : Type} (f : a -> b) (x : IO a),
-  bindIO x (fun a => returnIO (f a)) = fmapIO f x.
-
-Axiom fmapIO_id : forall {a : Type} (x : IO a),
-  fmapIO id x = x.
-
-Axiom unsafeDupablePerformIO : forall {a : Type}, IO a -> a.
-Axiom unsafeDupablePerformIO_inj : forall {a : Type} x y,
-  x = y -> @unsafeDupablePerformIO a x = unsafeDupablePerformIO y.
-
-Axiom unsafeDupablePerformIO_returnIO : forall {a : Type} (x : a),
-  unsafeDupablePerformIO (returnIO x) = x.
-
-Axiom malloc  : Size -> IO (Ptr Word).
-Axiom free    : Ptr Word -> IO ().
-Axiom realloc : Ptr Word -> Size -> IO (Ptr Word).
-Axiom peek    : Ptr Word -> IO Word.
-Axiom poke    : Ptr Word -> Word -> IO ().
-Axiom memcpy  : Ptr Word -> Ptr Word -> Size -> IO ().
-Axiom memset  : Ptr Word -> Size -> Word -> IO ().
-Axiom read    : Ptr Word -> Size -> IO (list Word).
-Axiom write   : Ptr Word -> list Word -> IO ().
-
-Definition ghcDenote {A : Type} : ClientDSL (getADTSig HeapSpec) (Rep HeapSpec) (IO A) -> IO A.
-Proof.
-  intros.
-  eapply (iter _) in X.
-  exact X.
-  Unshelve.
-  clear X.
-  destruct 1.
-  simpl in midx.
-  revert h y.
-  pattern midx; apply IterateBoundedIndex.Lookup_Iterate_Dep_Type;
-  simpl; repeat constructor; intros.
-
-  exact (y HeapState.newHeapState).
-  exact (bindIO (malloc (` (hlist_head (hlist_tail h))))
-                (y (hlist_head h))).
-  exact (bindIO (free (hlist_head (hlist_tail h)))
-                (fun _ => y (hlist_head h))).
-  exact (bindIO (realloc (hlist_head (hlist_tail h))
-                         (` (hlist_head (hlist_tail (hlist_tail h)))))
-                (y (hlist_head h))).
-  exact (bindIO (peek (hlist_head (hlist_tail h)))
-                (y (hlist_head h))).
-  exact (bindIO (poke (hlist_head (hlist_tail h))
-                      (hlist_head (hlist_tail (hlist_tail h))))
-                (fun _ => y (hlist_head h))).
-  exact (bindIO (memcpy (hlist_head (hlist_tail h))
-                          (hlist_head (hlist_tail (hlist_tail h)))
-                          (hlist_head (hlist_tail (hlist_tail (hlist_tail h)))))
-                (fun _ => y (hlist_head h))).
-  exact (bindIO (memset (hlist_head (hlist_tail h))
-                        (hlist_head (hlist_tail (hlist_tail h)))
-                        (hlist_head (hlist_tail (hlist_tail (hlist_tail h)))))
-                (fun _ => y (hlist_head h))).
-  exact (bindIO (read (hlist_head (hlist_tail h))
-                      (hlist_head (hlist_tail (hlist_tail h))))
-                (y (hlist_head h))).
-  exact (bindIO (write (hlist_head (hlist_tail h))
-                      (hlist_head (hlist_tail (hlist_tail h))))
-                (fun _ => y (hlist_head h))).
-Defined.
-
-Corollary bind_If `{Monad f} : forall A B (k : A -> f B) b t e,
-  ((If b Then t Else e) >>= k) = If b Then t >>= k Else e >>= k.
-Proof. destruct b; reflexivity. Qed.
-
-Corollary bind_IfDep `{Monad f} : forall A B (k : A -> f B) b t e,
-  ((IfDep b Then t Else e) >>= k) =
-  IfDep b Then (fun H => t H >>= k) Else (fun H => e H >>= k).
-Proof. destruct b; reflexivity. Qed.
-
-Corollary fmap_If `{Functor f} : forall A B (k : A -> B) b t e,
-  fmap k (If b Then t Else e) = If b Then fmap k t Else fmap k e.
-Proof. destruct b; reflexivity. Qed.
-
-Corollary fmap_IfDep `{Functor f} : forall A B (k : A -> B) b t e,
-  fmap k (IfDep b Then t Else e) =
-  IfDep b Then (fun H => fmap k (t H)) Else (fun H => fmap k (e H)).
-Proof. destruct b; reflexivity. Qed.
-
-Corollary iter_If `{Functor f} : forall A (phi : f A -> A) b t e,
-  iter phi (If b Then t Else e) = If b Then iter phi t Else iter phi e.
-Proof. destruct b; reflexivity. Qed.
-
-Corollary iter_IfDep `{Functor f} : forall A (phi : f A -> A) b t e,
-  iter phi (IfDep b Then t Else e) =
-  IfDep b Then (fun H => iter phi (t H)) Else (fun H => iter phi (e H)).
-Proof. destruct b; reflexivity. Qed.
-
-Corollary ghcDenote_If :
-  forall A b (t e : ClientDSL (getADTSig HeapSpec) (Rep HeapSpec) (IO A)),
-    ghcDenote (If b Then t Else e) = If b Then ghcDenote t Else ghcDenote e.
-Proof. destruct b; reflexivity. Qed.
-
-Corollary ghcDenote_IfDep :
-  forall b A (t : b = true -> ClientDSL (getADTSig HeapSpec) (Rep HeapSpec) (IO A))
-         (e : b = false -> ClientDSL (getADTSig HeapSpec) (Rep HeapSpec) (IO A)),
-    ghcDenote (IfDep b Then t Else e) = IfDep b Then ghcDenote \o t Else ghcDenote \o e.
-Proof. destruct b; reflexivity. Qed.
-
-Lemma ghcEmptyDSL :
-  { f : PS & f = unsafeDupablePerformIO (ghcDenote (returnIO <$> projT1 emptyDSL)) }.
-Proof.
-  eexists; intros.
-  symmetry.
-  unfold comp; simpl.
-  unfold ghcDenote; simpl.
-  rewrite unsafeDupablePerformIO_returnIO.
-  higher_order_reflexivity.
-Defined.
-
-Definition ghcEmptyDSL' := Eval simpl in projT1 ghcEmptyDSL.
-Print ghcEmptyDSL'.
-
-Lemma ghcPackDSL :
-  { f : list Word -> PS
-  & forall r xs,
-      f xs = unsafeDupablePerformIO
-               (ghcDenote ((returnIO \o fst) <$> projT1 (packDSL r xs))) }.
-Proof.
-  eexists; intros.
-  symmetry.
-  simpl projT1.
-  unfold comp.
-(*
-  rewrite !fmap_If.
-  etransitivity.
-    do 3 setoid_rewrite ghcDenote_If.
-    reflexivity.
-  simpl.
-  do 4 (unfold compose, comp; simpl).
-  unfold ghcDenote; simpl.
-  rewrite !bindIO_returnIO.
-  unfold If_Then_Else.
-  higher_order_reflexivity.
-Defined.
-*)
-Admitted.
-
-Definition ghcPackDSL' := Eval simpl in projT1 ghcPackDSL.
-Print ghcPackDSL'.
-
-Lemma ghcUnpackDSL :
-  { f : PS -> list Word
-  & forall r bs,
-      f bs = unsafeDupablePerformIO
-               (ghcDenote (returnIO <$> projT1 (unpackDSL r bs))) }.
-Proof.
-  eexists; intros.
-  symmetry.
-  simpl projT1.
-  unfold comp.
-  simpl.
-  do 4 (unfold compose, comp; simpl).
-  unfold ghcDenote; simpl.
-  rewrite !bindIO_returnIO, fmapIO_id.
-  higher_order_reflexivity.
-Defined.
-
-Definition ghcUnpackDSL' := Eval simpl in projT1 ghcUnpackDSL.
-Print ghcUnpackDSL'.
-
-Lemma ghcConsDSL :
-  { f : PS -> Word -> PS
-  & forall r bs w,
-      f bs w = unsafeDupablePerformIO
-                 (ghcDenote ((returnIO \o snd) <$> projT1 (consDSL r bs w))) }.
-Proof.
-  eexists; intros.
-  symmetry.
-  simpl projT1.
-  unfold comp.
-  rewrite !fmap_If.
-  etransitivity.
-    do 3 setoid_rewrite ghcDenote_If.
-    reflexivity.
-  simpl.
-  do 4 (unfold compose, comp; simpl).
-  unfold ghcDenote; simpl.
-  rewrite !bindIO_returnIO.
-  unfold If_Then_Else.
-  higher_order_reflexivity.
-Defined.
-
-Definition ghcConsDSL' := Eval simpl in projT1 ghcConsDSL.
-Print ghcConsDSL'.
-
-Lemma ghcUnconsDSL :
-  { f : PS -> PS * option Word
-  & forall r bs,
-      f bs = unsafeDupablePerformIO
-               (ghcDenote ((fun x => returnIO (snd (fst x), snd x))
-                             <$> projT1 (unconsDSL r bs))) }.
-Proof.
-  eexists; intros.
-  symmetry.
-  simpl projT1.
-  unfold comp.
-  simpl If_Then_Else.
-  rewrite !fmap_If.
-  etransitivity.
-    setoid_rewrite ghcDenote_If.
-    reflexivity.
-  simpl.
-  do 4 (unfold compose, comp; simpl).
-  unfold ghcDenote; simpl.
-  rewrite !bindIO_returnIO.
-  unfold If_Then_Else.
-  higher_order_reflexivity.
-Defined.
-
-Definition ghcUnconsDSL' := Eval simpl in projT1 ghcUnconsDSL.
-Print ghcUnconsDSL'.
-
-Lemma ghcAppendDSL :
-  { f : PS -> PS -> PS
-  & forall r1 bs1 bs2,
-      f bs1 bs2 = unsafeDupablePerformIO
-                    (ghcDenote ((returnIO \o snd)
-                                  <$> projT1 (appendDSL r1 bs1 bs2))) }.
-Proof.
-  eexists; intros.
-  symmetry.
-  simpl projT1.
-  unfold comp.
-  rewrite fmap_IfDep.
-  etransitivity.
-    setoid_rewrite ghcDenote_IfDep.
-    unfold comp.
-    apply unsafeDupablePerformIO_inj.
-    apply IfDep_Then_Else_fun_Proper; intro H.
-      rewrite fmap_IfDep.
-      apply ghcDenote_IfDep.
-    reflexivity.
-  simpl.
-  do 4 (unfold compose, comp; simpl).
-  unfold ghcDenote; simpl.
-  do 2 rewrite strip_IfDep_Then_Else.
-  unfold If_Then_Else.
-  higher_order_reflexivity.
-Defined.
-
-Definition ghcAppendDSL' := Eval simpl in projT1 ghcAppendDSL.
-Print ghcAppendDSL'.
-
 End ByteStringFFI.
-
-(****************************************************************************
-
-This is the code we intend to approximate with the FFI refined version of
-ByteString:
-
-  import Data.Word8
-  import GHC.ForeignPtr
-  import GHC.IO
-
-  data ByteString = PS {-# UNPACK #-} !(ForeignPtr Word8) -- payload
-                       {-# UNPACK #-} !Int                -- offset
-                       {-# UNPACK #-} !Int                -- length
-      deriving (Typeable)
-
-  {--[ cons ]---------------------------------------------------------------}
-
-  mallocByteString :: Int -> IO (ForeignPtr a)
-  mallocByteString l = GHC.mallocPlainForeignPtrBytes l
-
-  create :: Int -> (Ptr Word8 -> IO ()) -> IO ByteString
-  create l f = do
-      fp <- mallocByteString l
-      withForeignPtr fp $ \p -> f p
-      return $! PS fp 0 l
-
-  unsafeCreate :: Int -> (Ptr Word8 -> IO ()) -> ByteString
-  unsafeCreate l f = unsafeDupablePerformIO (create l f)
-
-  foreign import ccall unsafe "string.h memcpy" c_memcpy
-      :: Ptr Word8 -> Ptr Word8 -> CSize -> IO (Ptr Word8)
-
-  memcpy :: Ptr Word8 -> Ptr Word8 -> Int -> IO ()
-  memcpy p q s = c_memcpy p q (fromIntegral s) >> return ()
-
-  cons :: Word8 -> ByteString -> ByteString
-  cons c (PS x s l) = unsafeCreate (l+1) $ \p -> withForeignPtr x $ \f -> do
-          poke p c
-          memcpy (p `plusPtr` 1) (f `plusPtr` s) (fromIntegral l)
-
-  {--[ uncons ]-------------------------------------------------------------}
-
-  accursedUnutterablePerformIO :: IO a -> a
-  accursedUnutterablePerformIO (IO m) = case m realWorld# of (# _, r #) -> r
-
-  uncons :: ByteString -> Maybe (Word8, ByteString)
-  uncons (PS x s l)
-      | l <= 0    = Nothing
-      | otherwise = Just (accursedUnutterablePerformIO $ withForeignPtr x
-                                                       $ \p -> peekByteOff p s,
-                          PS x (s+1) (l-1))
-
-****************************************************************************)
